Pool: introduce task_spotted
This simplifies some lemmas significantly and removes the admit in the
worker loop by observing that the task, and not the handle, was exactly
present in the pool at some point.

share/pulse/examples/NuPool.fst
@@ -210,67 +210,81 @@ let state_res' #code (post : erased code.t) ([@@@equate_by_smt] st : task_state 
   | Claimed -> emp
   | _ -> pure False
 
-let handle_in_task_list
-  (#code:vcode) (#post : erased code.t)
-  (h : handle post)
-  (ts : list (task_t code))
-  : prop
-  =
-  exists (task : task_t code).
-    task.post == post
-    /\ task.h == h
-    /\ List.memP task ts
+let task_spotted (#code:vcode)
+  (p : pool code)
+  (t : task_t code)
+: vprop =
+  exists* v_runnable.
+    BAR.snapshot p.g_runnable v_runnable **
+    pure (List.memP t v_runnable)
 
+// TODO: rename to handle_spotted
 let snapshot_mem (#code:vcode)
   (p : pool code)
   (#[@@@equate_by_smt]post : erased code.t)
   (h : handle post)
-: vprop =
-  exists* v_runnable.
-    BAR.snapshot p.g_runnable v_runnable **
-    pure (handle_in_task_list h v_runnable)
+  : vprop =
+    exists* (t : task_t code).
+      task_spotted p t **
+      pure (t.post == post /\ t.h == h)
+
+```pulse
+ghost
+fn intro_task_spotted
+    (#code:vcode) (p : pool code)
+    (t : task_t code)
+    (ts : list (task_t code))
+  requires BAR.snapshot p.g_runnable ts
+        ** pure (List.memP t ts)
+  ensures  task_spotted p t
+{
+  fold (task_spotted p t);
+}
+```
 
 ```pulse
 ghost
 fn intro_snapshot_mem
     (#code:vcode) (p : pool code)
-    (#post:erased code.t) (h : handle post)
-    (task : task_t code)
+    (t : task_t code)
     (ts : list (task_t code))
   requires BAR.snapshot p.g_runnable ts
-      ** pure (task.post == post /\ task.h == h /\ List.memP task ts)
-  ensures  snapshot_mem p h
+        ** pure (List.memP t ts)
+  ensures  snapshot_mem p t.h
 {
-  fold (snapshot_mem p h);
+  intro_task_spotted #code p t ts;
+  fold (snapshot_mem p t.h);
 }
 ```
 
-let handle_in_task_list_mono
-    (#code:vcode) (#post:erased code.t)
-    (h : handle post) (ts1 ts2 : list (task_t code))
-: Lemma (requires list_preorder ts1 ts2 /\ handle_in_task_list h ts1)
-        (ensures handle_in_task_list h ts2)
-=
-  assume (forall x. List.memP x ts1 ==> List.memP x ts2); // should follow from list_preorder
-  ()
+// let handle_in_task_list_mono
+//     (#code:vcode) (#post:erased code.t)
+//     (h : handle post) (ts1 ts2 : list (task_t code))
+// : Lemma (requires list_preorder ts1 ts2 /\ handle_in_task_list h ts1)
+//         (ensures handle_in_task_list h ts2)
+// =
+//   assume (forall x. List.memP x ts1 ==> List.memP x ts2); // should follow from list_preorder
+//   ()
+
+let list_preorder_mono_memP (#a:Type) (x:a) (l1 l2:list a)
+  : Lemma (requires List.memP x l1 /\ list_preorder l1 l2)
+          (ensures List.memP x l2)
+          [SMTPat (list_preorder l1 l2); SMTPat (List.memP x l1)]
+      = admit()
 
 ```pulse
 ghost
-fn recall_snapshot_mem0
-  (#code:vcode) (p : pool code) (#post : erased code.t) (h : handle post) (#ts : list (task_t code))
-  requires BAR.pts_to_full p.g_runnable ts ** snapshot_mem p h
-  ensures  BAR.pts_to_full p.g_runnable ts ** snapshot_mem p h **
-            pure (handle_in_task_list h ts)
+fn recall_task_spotted
+  (#code:vcode) (p : pool code) (t : task_t code) (#ts : list (task_t code))
+  requires BAR.pts_to_full p.g_runnable ts ** task_spotted p t
+  ensures  BAR.pts_to_full p.g_runnable ts ** task_spotted p t
+           ** pure (List.memP t ts)
 {
-  unfold (snapshot_mem p h);
-  with ts0. assert (BAR.snapshot p.g_runnable ts0);
+  unfold (task_spotted p t);
   BAR.drop_anchor p.g_runnable;
   BAR.recall_snapshot p.g_runnable;
-  BAR.lift_anchor p.g_runnable _;
-  assert (pure (handle_in_task_list h ts0));
-  handle_in_task_list_mono #code #post h ts0 ts;
-  assert (pure (handle_in_task_list h ts));
-  fold (snapshot_mem p h);
+  BAR.lift_anchor p.g_runnable ts;
+  fold (task_spotted p t);
 }
 ```
 
@@ -292,25 +306,13 @@ fn recall_snapshot_mem
   requires BAR.pts_to_full p.g_runnable ts ** snapshot_mem p h
   returns  task : erased (task_t code)
   ensures  BAR.pts_to_full p.g_runnable ts ** snapshot_mem p h **
-            pure (task.post == post /\ task.h == h /\ List.memP (reveal task) ts /\
-                  handle_in_task_list h ts)
+            pure (task.post == post /\ task.h == h /\ List.memP (reveal task) ts)
 {
   unfold (snapshot_mem p h);
-  with ts0. assert (BAR.snapshot p.g_runnable ts0);
-  BAR.drop_anchor p.g_runnable;
-  BAR.recall_snapshot p.g_runnable;
-  BAR.lift_anchor p.g_runnable ts;
-  assert (pure (list_preorder ts0 ts /\ True));
-  assert (pure (handle_in_task_list h ts0));
+  with t. assert (task_spotted p t);
+  recall_task_spotted #code p t #ts;
   fold (snapshot_mem p h);
-  assert (pure (handle_in_task_list h ts0));
-  assert (pure (exists (task : task_t code). 
-      (task.post == post /\ task.h == h /\ List.memP task ts0)));
-  let task = elim_exists_explicit (fun (task : task_t code) ->
-      (task.post == post /\ task.h == h /\ List.memP task ts0));
-      ();
-  mem_lemma task ts0 ts;
-  hide task
+  hide t
 }
 ```
 
@@ -335,26 +337,26 @@ fn star_to_trade (p q : vprop)
 module SEM = FStar.StrongExcludedMiddle
 
 ```pulse
-ghost // or concrete?
+ghost
 fn rec extract_state_pred
   (#code:vcode)
-  (p : pool code) (#post:code.t) (h : handle post)
+  (p : pool code) (t : task_t code)
   (#ts : list (task_t code))
-  requires all_state_pred ts ** pure (handle_in_task_list h ts)
-  returns task : erased (task_t code)
-  ensures pure (task.post == post /\ task.h == h /\ List.memP (reveal task) ts)
-       ** state_pred task.pre task.post task.h
-       ** trade (state_pred task.pre task.post task.h) (all_state_pred ts) // trade to put things back togtaskher
+  requires all_state_pred ts ** pure (List.memP t ts)
+  ensures state_pred t.pre t.post t.h
+       ** trade (state_pred t.pre t.post t.h) (all_state_pred ts) // trade to put things back together
   decreases ts
 {
   open Pulse.Lib.InvList;
   match ts {
-    Nil -> { unreachable () }
+    Nil -> {
+      unreachable ()
+    }
     Cons t' ts' -> {
-      let b = SEM.strong_excluded_middle (t'.post == post /\ t'.h == h /\ List.memP t' ts);
+      let b = SEM.strong_excluded_middle (t == t');
       if not b {
         take_one_h11 t' ts';
-        let ret = extract_state_pred p h #ts';
+        extract_state_pred p t #ts';
 
         ghost
         fn aux (_:unit)
@@ -368,12 +370,10 @@ fn rec extract_state_pred
         intro_trade (all_state_pred ts') (all_state_pred ts)
                     (state_pred t'.pre t'.post t'.h) aux;
 
-        trade_compose (state_pred ret.pre ret.post ret.h) (all_state_pred ts') (all_state_pred ts);
-
-        ret
+        trade_compose (state_pred t.pre t.post t.h) (all_state_pred ts') (all_state_pred ts);
       } else {
-        let ret = hide t';
-        take_one_h11 t' ts';
+        rewrite each t' as t;
+        take_one_h11 t ts';
 
         ghost
         fn aux (_:unit)
@@ -383,10 +383,10 @@ fn rec extract_state_pred
         {
           add_one_state_pred t' ts';
         };
-        intro_trade (state_pred ret.pre ret.post ret.h) (all_state_pred ts)
+        intro_trade (state_pred t.pre t.post t.h) (all_state_pred ts)
                     (pure (ts == t'::ts') ** all_state_pred ts') aux;
 
-        ret
+        ()
       }
     }
   }
@@ -568,15 +568,14 @@ fn spawn' (code:vcode) (p:pool code)
   rewrite each task_st as (Ready #code #post);
   rewrite each gr_task_st as task.h.g_state;
   assert (BAR.anchored task.h.g_state (Ready #code #post));
-  
 
   BAR.take_snapshot' p.g_runnable;
   
   assert (pure (List.memP task (task :: v_runnable)));
-  intro_snapshot_mem p task.h task (task :: v_runnable);
+  // intro_task_spotted p task (task :: v_runnable);
+  intro_snapshot_mem p task (task :: v_runnable);
 
   fold (joinable #code p post task.h);
-
 
   fold (pool_alive #pf p);
   
@@ -654,36 +653,26 @@ fn try_await
   returns  ok : bool
   ensures  pool_alive #f p ** (if ok then code.up post else joinable p post h)
 {
-  unfold (joinable p post h);
-
   unfold (pool_alive #f p);
   acquire p.lk;
   unfold (lock_inv p.runnable p.g_runnable);
   
+  unfold (joinable p post h);
+
   with v_runnable. assert (Big.pts_to p.runnable v_runnable);
 
-  // let task = recall_snapshot_mem #code p #post h #v_runnable;
-  // ^fails: ill-typed substitution or solver could not prove uvar
-  // let task : erased (task_t code) = magic u#2 #(erased (task_t code)) ();
-  // assume_ (pure (task.post == post /\ task.h == h /\ List.memP (reveal task) v_runnable));
+  unfold (snapshot_mem p h);
 
-  assert (BAR.pts_to_full p.g_runnable v_runnable);
-  assert (snapshot_mem p h);
+  with t. assert (task_spotted p t);
+  recall_task_spotted #code p t #v_runnable;
   
-  recall_snapshot_mem0 #code p #post h #v_runnable;
-
-  // recall_snapshot_mem #code p #post h #v_runnable;
-  // - Tactic logged issue:
-  // - prover error: ill-typed substitutions (prover could not prove uvar _#11)
-  
-  assert (pure (handle_in_task_list h v_runnable));
-  let task = extract_state_pred p h #v_runnable;
+  extract_state_pred p t #v_runnable;
 
   // assume_ (pure (post == task.post)); // fixme: core ref construction
 
-  let v_state = elim_state_pred task.pre task.post task.h;
-  
-  rewrite (Big.pts_to task.h.state #(if Running? v_state then half_perm full_perm else full_perm) (unclaimed (reveal v_state)))
+  let v_state = elim_state_pred t.pre t.post t.h;
+
+  rewrite (Big.pts_to t.h.state #(if Running? v_state then half_perm full_perm else full_perm) (unclaimed (reveal v_state)))
        as (Big.pts_to h.state #(if Running? v_state then half_perm full_perm else full_perm) (unclaimed (reveal v_state)));
   let task_st = Big.op_Bang h.state;
   
@@ -691,31 +680,33 @@ fn try_await
     Ready -> {
       (* NOOP *)
       rewrite (Big.pts_to h.state (reveal v_state))
-           as (Big.pts_to task.h.state (reveal v_state));
-      intro_state_pred task.pre task.post task.h Ready;
+           as (Big.pts_to t.h.state (reveal v_state));
+      intro_state_pred t.pre t.post t.h Ready;
       elim_trade _ _; // undo extract_state_pred
       fold (lock_inv p.runnable p.g_runnable);
       release p.lk;
       fold (pool_alive #f p);
+      fold (snapshot_mem p h);
       fold (joinable p post h);
       false;
     }
     Running -> {
       (* NOOP *)
       rewrite (Big.pts_to h.state #(half_perm full_perm) (reveal v_state))
-           as (Big.pts_to task.h.state #(half_perm full_perm) (reveal v_state));
-      intro_state_pred_Running task.pre task.post task.h;
+           as (Big.pts_to t.h.state #(half_perm full_perm) (reveal v_state));
+      intro_state_pred_Running t.pre t.post t.h;
       elim_trade _ _; // undo extract_state_pred
       fold (lock_inv p.runnable p.g_runnable);
       release p.lk;
       fold (pool_alive #f p);
+      fold (snapshot_mem p h);
       fold (joinable p post h);
       false;
     }
     Done -> {
       (* First prove that ghost state cannot be Claimed,
       due to the anchor *)
-      rewrite (BAR.pts_to task.h.g_state v_state)
+      rewrite (BAR.pts_to t.h.g_state v_state)
            as (BAR.pts_to h.g_state v_state);
       assert (BAR.pts_to h.g_state v_state);
       assert (BAR.anchored h.g_state Ready);
@@ -723,22 +714,22 @@ fn try_await
       assert (pure (v_state =!= Claimed));
       assert (pure (v_state == Done));
       rewrite (BAR.pts_to h.g_state v_state)
-           as (BAR.pts_to task.h.g_state v_state);
+           as (BAR.pts_to t.h.g_state v_state);
 
       (* Now claim it *)
-      claim_done_task #code #p #task.pre #task.post task.h;
+      claim_done_task #code #p #t.pre #t.post t.h;
 
       rewrite (code.up post)
            as (if true then code.up post else joinable p post h);
            
       rewrite (Big.pts_to h.state Done)
-           as (Big.pts_to task.h.state (unclaimed Claimed));
-      intro_state_pred task.pre task.post task.h Claimed;
+           as (Big.pts_to t.h.state (unclaimed Claimed));
+      intro_state_pred t.pre t.post t.h Claimed;
       elim_trade _ _; // undo extract_state_pred
       fold (lock_inv p.runnable p.g_runnable);
       release p.lk;
       fold (pool_alive #f p);
-      drop_ (snapshot_mem p h);
+      drop_ (task_spotted p t);
       true
     }
     Claimed -> {
@@ -789,36 +780,37 @@ fn disown_aux
   unfold (handle_done h);
   unfold (lock_inv p.runnable p.g_runnable);
   unfold (joinable p post h);
+  unfold (snapshot_mem p h);
 
   with v_runnable. assert (Big.pts_to p.runnable v_runnable);
+  with t. assert (task_spotted p t);
 
-  (* FIXME: calling recall_snapshot_mem (not the 0 version) fails *)
-  recall_snapshot_mem0 #code p #post h #v_runnable;
-  let et = extract_state_pred p h #v_runnable;
+  recall_task_spotted #code p t #v_runnable;
+  extract_state_pred p t #v_runnable;
 
-  unfold (state_pred et.pre et.post et.h);
+  unfold (state_pred t.pre t.post t.h);
 
-  with st. assert (BAR.pts_to et.h.g_state st);
+  with st. assert (BAR.pts_to t.h.g_state st);
   let st = reveal st;
 
   match st {
     Done -> {
-      rewrite (state_res et.pre et.post et.h.g_state Done)
+      rewrite (state_res t.pre t.post t.h.g_state Done)
            as code.up post;
 
-      BAR.lift_anchor et.h.g_state Ready;
-      BAR.write_full et.h.g_state Claimed;
-      BAR.drop_anchor et.h.g_state;
+      BAR.lift_anchor t.h.g_state Ready;
+      BAR.write_full t.h.g_state Claimed;
+      BAR.drop_anchor t.h.g_state;
 
-      fold (state_res et.pre et.post et.h.g_state Claimed);
+      fold (state_res t.pre t.post t.h.g_state Claimed);
       
-      rewrite (Big.pts_to et.h.state Done)
-           as (Big.pts_to et.h.state (unclaimed Claimed));
+      rewrite (Big.pts_to t.h.state Done)
+           as (Big.pts_to t.h.state (unclaimed Claimed));
       
-      intro_state_pred et.pre et.post et.h Claimed;
+      intro_state_pred t.pre t.post t.h Claimed;
 
       fold (handle_done h);
-      drop_ (snapshot_mem p h);
+      drop_ (task_spotted p t);
       
       elim_trade_ghost _ _;
       
@@ -828,17 +820,17 @@ fn disown_aux
     }
     Claimed -> {
       assert (BAR.anchored h.g_state Ready);
-      BAR.recall_anchor et.h.g_state Ready;
+      BAR.recall_anchor t.h.g_state Ready;
       unreachable();
     }
     Ready -> {
-      rewrite (BAR.pts_to et.h.g_state Ready)
+      rewrite (BAR.pts_to t.h.g_state Ready)
            as BAR.pts_to h.g_state Ready;
       BAR.recall_snapshot h.g_state;
       unreachable();
     }
     Running -> { 
-      rewrite (BAR.pts_to et.h.g_state Running)
+      rewrite (BAR.pts_to t.h.g_state Running)
            as BAR.pts_to h.g_state Running;
       BAR.recall_snapshot h.g_state;
       unreachable();
@@ -873,14 +865,36 @@ let pool_done (#code:vcode) (p : pool code) : vprop =
 
 ```pulse
 ghost
+fn __pool_done_handle_done_aux2 (#code:vcode) (#p:pool code)
+      (#post : erased code.t)
+      (h : handle post)
+      (ts : list (task_t code))
+  requires pool_done_fa p ts 
+  ensures  pool_done_fa p ts ** handle_done h
+{
+  match ts {
+    Nil -> {
+      admit(); // should be impossible, handle must be in ts
+    }
+    Cons t ts' -> {
+      admit();
+    }
+  }
+}
+```
+
+```pulse
+ghost
 fn __pool_done_handle_done (#code:vcode) (#p:pool code)
       (#post : erased code.t)
       (h : handle post)
       (_ : unit)
-  requires invlist_v invlist_empty ** (pool_done p ** emp)
-  ensures  invlist_v invlist_empty ** (pool_done p ** handle_done h)
+  requires emp ** (pool_done p ** emp)
+  ensures  emp ** (pool_done p ** handle_done h)
 {
-  admit();
+  unfold (pool_done p);
+  __pool_done_handle_done_aux2 #code #p #post h _;
+  fold (pool_done p);
 }
 ```
 
@@ -918,7 +932,7 @@ fn rec grab_work' (#code:vcode) (p:pool code)
   returns  topt : option (task_t code)
   ensures  lock_inv p.runnable p.g_runnable
         ** vopt topt (fun t ->
-             code.up t.pre ** Big.pts_to t.h.state #(half_perm full_perm) Running ** snapshot_mem p t.h)
+             code.up t.pre ** Big.pts_to t.h.state #(half_perm full_perm) Running ** task_spotted p t)
 {
   unfold (lock_inv p.runnable p.g_runnable);
   with v_runnable. assert (Big.pts_to p.runnable v_runnable);
@@ -949,15 +963,15 @@ fn rec grab_work' (#code:vcode) (p:pool code)
           Big.share2 t.h.state;
 
           BAR.take_snapshot' p.g_runnable;
-          intro_snapshot_mem p #t.post t.h t v_runnable;
+          intro_task_spotted p t v_runnable;
 
           intro_state_pred_Running t.pre t.post t.h;
           add_one_state_pred t ts;
           fold (lock_inv p.runnable p.g_runnable);
 
           
-          rewrite code.up t.pre ** Big.pts_to t.h.state #(half_perm full_perm) Running ** snapshot_mem p t.h
-               as vopt topt (fun t -> code.up t.pre ** Big.pts_to t.h.state #(half_perm full_perm) Running ** snapshot_mem p t.h);
+          rewrite code.up t.pre ** Big.pts_to t.h.state #(half_perm full_perm) Running ** task_spotted p t
+               as vopt topt (fun t -> code.up t.pre ** Big.pts_to t.h.state #(half_perm full_perm) Running ** task_spotted p t);
           
           topt
         }
@@ -977,7 +991,7 @@ fn grab_work (#code:vcode) (p:pool code)
   returns  topt : option (task_t code)
   ensures  pool_alive #f p
         ** vopt topt (fun t ->
-             code.up t.pre ** Big.pts_to t.h.state #(half_perm full_perm) Running ** snapshot_mem p t.h)
+             code.up t.pre ** Big.pts_to t.h.state #(half_perm full_perm) Running ** task_spotted p t)
 {
   unfold (pool_alive #f p);
   acquire p.lk;
@@ -1002,17 +1016,15 @@ fn perf_work (#code:vcode) (t : task_t code)
 ```pulse
 fn put_back_result (#code:vcode) (p:pool code) (t : task_t code)
   requires pool_alive #f p **
-           snapshot_mem p t.h **
+           task_spotted p t **
            code.up t.post **
            Big.pts_to t.h.state #(half_perm full_perm) Running
   ensures  pool_alive #f p
 {
   acquire p.lk;
   unfold (lock_inv p.runnable p.g_runnable);
-  recall_snapshot_mem p t.h;
-  let t' = extract_state_pred p t.h;
-  assume_ (pure (t == t')); // FIXME: change snapshot_mem to speak about tasks and not handles
-  rewrite each t' as t;
+  recall_task_spotted p t;
+  extract_state_pred p t;
 
   (* Advance the state and place the post condition back into the pool *)
   assert (state_pred t.pre t.post t.h ** Big.pts_to t.h.state #(half_perm full_perm) Running);
@@ -1037,10 +1049,9 @@ fn put_back_result (#code:vcode) (p:pool code) (t : task_t code)
 
   fold (lock_inv p.runnable p.g_runnable);
   release p.lk;
-  drop_ (snapshot_mem p t.h);
+  drop_ (task_spotted p t);
 }
 ```
-
 
 ```pulse
 fn rec worker (#code:vcode) (#f:perm) (p : pool code)
@@ -1058,8 +1069,8 @@ fn rec worker (#code:vcode) (#f:perm) (p : pool code)
       rewrite each topt as Some t;
       get_vopt #(task_t code) #t ();
       (* sigh *)
-      rewrite (fun t -> code.up t.pre ** Big.pts_to t.h.state #(half_perm full_perm) Running ** snapshot_mem p t.h) t
-           as code.up t.pre ** Big.pts_to t.h.state #(half_perm full_perm) Running ** snapshot_mem p t.h;
+      rewrite (fun t -> code.up t.pre ** Big.pts_to t.h.state #(half_perm full_perm) Running ** task_spotted p t) t
+           as code.up t.pre ** Big.pts_to t.h.state #(half_perm full_perm) Running ** task_spotted p t;
       perf_work t;
       put_back_result p t;
       worker p
